stronger invariant that enforces uniqueness, get and add

examples/JahobAssocList.v
@@ -12,13 +12,11 @@ Module NondepAssocListModel(A : NONDEP_ASSOCIATION).
  Require Export List.
  Set Implicit Arguments.
 
- Check fold_left.
-
  Fixpoint update l (k: K) (v: V)  :=
    match l with
      | nil => nil
      | (k', v')::b => if eqK k k' then (k, v) :: b else (k', v') :: update b k v
-    end.
+   end.
 
  Fixpoint delete (l: list (prod K V)) (k: K) :=
   match l with
@@ -39,10 +37,7 @@ Module NondepAssocListModel(A : NONDEP_ASSOCIATION).
    end.
 End NondepAssocListModel.
 
-(* This is the interface for the Jahob AssocList example.
-   (Minus containsKey, which is essentially a duplicate of get).
-   Specs are written using the 'operational' definitions
-   above rather than set theory. *)
+(* This is the interface for the Jahob AssocList example. *)
 Module Type JAHOB_ASSOC_LIST.
  Require Export List.
  Declare Module A  : NONDEP_ASSOCIATION.
@@ -103,10 +98,10 @@ Module JahobAssocList(A : NONDEP_ASSOCIATION) : JAHOB_ASSOC_LIST with Module A :
 
   Fixpoint rep' m (op: option ptr) {struct m} :=
     match op with
-      | None => [m = nil]
+      | None => [m = nil] 
       | Some h => match m with
-                    | (k,v) :: b => 
-                        Exists nxt :@ option ptr, 
+                    | (k,v) :: b => [lookup b k = None] * 
+                        Exists nxt :@ option ptr,
                           h --> node k v nxt * rep' b nxt
                     | nil => [False]
                    end
@@ -117,6 +112,13 @@ Module JahobAssocList(A : NONDEP_ASSOCIATION) : JAHOB_ASSOC_LIST with Module A :
 
 (* Reasoning **************************************************)
 
+ Lemma nilrep : forall m k, 
+  rep' m None ==> rep' m None * [lookup m k = None].
+   intros. destruct m. sep fail auto. simpl. assert (p :: m = nil -> False).
+   discriminate. sep fail auto. Defined.
+
+ Hint Resolve nilrep.
+
  Lemma eta_node : forall fn, fn = node (key fn) (value fn) (next fn).
    destruct fn; reflexivity.
   Qed.
@@ -125,7 +127,8 @@ Module JahobAssocList(A : NONDEP_ASSOCIATION) : JAHOB_ASSOC_LIST with Module A :
   Lemma eta_node2 : forall fn a b, 
    Some (a, b) = Some (key fn, value fn) -> 
    fn = node a b (next fn).
-    intros fn a b pf; assert (a = key fn); try congruence; assert (b = value fn); try congruence; subst; apply eta_node. 
+    intros fn a b pf; assert (a = key fn); try congruence; 
+   assert (b = value fn); try congruence; subst; apply eta_node. 
   Qed.
   Hint Resolve eta_node2.
 
@@ -142,7 +145,8 @@ Module JahobAssocList(A : NONDEP_ASSOCIATION) : JAHOB_ASSOC_LIST with Module A :
            end ==> _] ] => destruct v  
     | [ H : _ :: _ = _ :: _ |- _ ] => injection H; clear H; intros; subst
     | [ |- context[ if (eqK ?v1 ?v2) then _ else _ ] ] => destruct (eqK v1 v2)
-    | [ H : Specif.value ?a = Some ?b |- _ ] =>  unfold Specif.value in H; assert (a = b); congruence 
+    | [ H : Specif.value ?a = Some ?b |- _ ] =>  
+          unfold Specif.value in H; assert (a = b); congruence 
   end).
 
  Ltac printGoal := match goal with [ |- ?g ] => idtac g end.
@@ -150,54 +154,61 @@ Module JahobAssocList(A : NONDEP_ASSOCIATION) : JAHOB_ASSOC_LIST with Module A :
  Ltac t := unfold rep; unfold rep'; try congruence; try subst; sep fail simplr.
  Ltac f := fold rep'; fold rep.
 
+ Lemma reprev : forall hd0 m,
+   rep' m (Some hd0) ==> Exists n :@ Node,
+   [head m = Some (key n, value n)] * hd0 --> n *
+   rep' (tail m) (next n). 
+ intros. destruct m. t. t. Defined.
+
 
 (* Implementation ***************************************************)
 
   Open Scope stsepi_scope.
 
   Definition new : STsep __ (rep nil).
-    refine {{ New (@None ptr) }};
-      t.
-  Qed.
+    refine {{ New (@None ptr) }}; t. Qed.
 
   Definition free  p: STsep (rep nil p) (fun _:unit => __).
-  intros; refine {{ Free p }}; 
-     t.
-  Qed.  
+  intros; refine {{ Free p }}; t. Qed.  
 
-  Definition get'' (k: K) (hd: option ptr) (m: [list (prod K V)]):
+Parameter ff: False.
+
+
+Definition get'' (k: K) (hd: option ptr) (m: [list (prod K V)]):
     STsep (m ~~ rep' m hd) (fun r => m ~~ [r = lookup m k] * rep' m hd).
   intro k.
   refine (Fix2
     (fun hd m => m ~~ rep' m hd)
     (fun hd m o => m ~~ [o = lookup m k] * rep' m hd)
-    (fun self hd m =>
-      IfNull hd 
-      Then {{ Return None }}
-      Else  Assert (m ~~ Exists fn :@ Node, [head m = Some (key fn, value fn)] * hd --> fn * rep' (tail m) (next fn)) ;; 
-            fn <- !hd ;     
-            if eqK (key fn) k  
-            then {{ Return (Some (value fn)) }} 
-            else {{ self (next fn) (m ~~~ tail m) <@> (m ~~ hd --> fn * [head m = Some (key fn, value fn)]) }} 
-      ));  try solve [ t | repeat (hdestruct m; t) ]. Defined.
+    (fun self : forall hd m, STsep (m ~~ rep' m hd) (fun r => m ~~ [r = lookup m k] * rep' m hd) => fun hd m => 
+      IfNull hd
+      Then  Assert (m ~~ [m = nil]) ;;
+            {{ Return None }}
+      Else  fn <- SepRead hd (fun fn => m ~~  [head m = Some (key fn, value fn)] * 
+                                              rep' (tail m) (next fn) *
+                                              [lookup (tail m) (key fn) = None] *
+                                              [lookup m (key fn) = Some (value fn)] );
+            if eqK (key fn) k 
+            then {{ Return (Some (value fn)) 
+                     <@>              (hd --> fn * (m ~~ 
+                                              [head m = Some (key fn, value fn)] * 
+                                              rep' (tail m) (next fn)  *
+                                              [lookup (tail m) (key fn) = None] *    
+                                              [lookup m k = Some (value fn)] ))  }}  
+            else {{ self (next fn) (m ~~~ tail m) 
+                     <@>             (hd --> fn * (m ~~  
+                                              [head m = Some (key fn, value fn)] * 
+                                              [lookup (tail m) (key fn) = None] )) }} ));
+try solve [ t | repeat (hdestruct m; t) ]. Qed.
+
 
   Definition get (k: K) (p: ptr) (m: [list (prod K V)]) :
     STsep (m ~~ rep m p)
           (fun r:option V => m ~~ [r = lookup m k] * rep m p ).
   intros; refine (hd <- !p;
                   Assert (p --> hd * (m ~~ rep' m hd));;
-                  {{get'' k hd m <@> _}});
-    t. Defined. 
+                  {{get'' k hd m <@> _}}); t. Qed.
 
- (* This will verify even without the lookup m k = None
-    condition.  Rather than 'bake in' the uniqueness of keys into
-    the heap invariant we can instead only expose operations
-    that preserve this additional property.  However, I think
-    this might be cheating because you can't take an arbitary
-    pointer satisfying the invariant and claim that it actually
-    models an association list without also knowing that 
-    nothing else has messed it up.  So I need to go back and
-    change the invariant. *)    
  Definition add: forall k v (p: t) (m: [list (prod K V)]),
   STsep (m ~~ rep m p * [lookup m k = None])
         (fun _:unit => m ~~ rep ((k,v)::m) p).
@@ -220,10 +231,9 @@ Module JahobAssocList(A : NONDEP_ASSOCIATION) : JAHOB_ASSOC_LIST with Module A :
  Conjecture isEmpty: forall (p: t) (m: [list (prod K V)]),
    STsep (m ~~ rep m p) (fun r:bool => m ~~ rep m p * if r then [m = nil] else [m <> nil]).
 
-
  (* The Jahob put operation traverses the list several times.  
     This implements a faster, in-place put that isn't found in Jahob. *)
-
+(* This hasn't been updated for the uniqueness part of the invariant 
  Definition putFast' (k: K) (v: V) (hdptr: ptr) (m: [list (prod K V)]) :
   STsep (m ~~ rep' m (Some hdptr))
         (fun r => m ~~ [r = lookup m k] * rep' (insert m k v) (Some hdptr)).
@@ -255,6 +265,8 @@ intros; refine(
         {{ Return None }}
    Else {{ putFast' k v opthd m <@> _ }} );
  try solve [ t | progress (hdestruct m; t) | destruct fn; hdestruct m; t; destruct m; t; t ]. Defined.
+
+*)
 
 End JahobAssocList.
 
